Refine assert/infeasibility handling a bit

src/tools/symbexec/birs_rulesScript.sml
@@ -8,12 +8,64 @@ open symb_recordTheory;
 open bir_symbTheory;
 open bir_symb_sound_coreTheory;
 
+open symb_typesLib;
 open HolBACoreSimps;
 
 val birs_state_ss = rewrites (type_rws ``:birs_state_t``);
 
 val _ = new_theory "birs_rules";
 
+
+
+val birs_pcondinf_def = Define `
+    birs_pcondinf pcond =
+  (!H.
+    (birs_interpr_welltyped H) ==>
+    (symb_interpr_for_symbs (bir_vars_of_exp pcond) H) ==>
+    (birs_interpret_fun H pcond = SOME bir_val_false)
+  )
+`;
+
+(*
+val birs_interpret_fun_NOT_true_thm = store_thm(
+   "birs_interpret_fun_NOT_true_thm", ``
+!H bexp.
+  (birs_interpr_welltyped H) ==>
+  (symb_interpr_for_symbs (bir_vars_of_exp bexp) H) ==>
+
+  (birs_interpret_fun H bexp <> SOME bir_val_true) ==>
+  (birs_interpret_fun H bexp = SOME bir_val_false)
+``,
+  cheat
+);
+*)
+
+
+val birs_pcondinf_thm = store_thm(
+   "birs_pcondinf_thm", ``
+!bprog sys.
+  birs_pcondinf (symb_symbst_pcond sys) ==>
+  symb_pcondinf (bir_symb_rec_sbir bprog) sys
+``,
+  REWRITE_TAC [symb_rulesTheory.symb_pcondinf_def, birs_pcondinf_def] >>
+  REWRITE_TAC [birs_interpr_welltyped_EQ_thm] >>
+  SIMP_TAC (std_ss++symb_TYPES_ss) [bir_symb_rec_sbir_def, symb_interpr_symbpcond_def, bir_bool_expTheory.bir_val_TF_dist]
+);
+
+(* TODO: unify pcondinf and simplification_e and integrate similarly in symb_pcondwiden *)
+(*
+val birs_interpret_fun_AND_IMP_true_thm = store_thm(
+   "birs_interpret_fun_NOT_true_thm", ``
+!H bexp.
+  (birs_interpr_welltyped H) ==>
+  (symb_interpr_for_symbs (bir_vars_of_exp bexp) H) ==>
+
+  (birs_interpret_fun H bexp <> SOME bir_val_true) ==>
+  (birs_interpret_fun H bexp = SOME bir_val_false)
+``,
+  cheat
+);
+*)
 
 val assert_spec_thm = store_thm(
    "assert_spec_thm", ``
@@ -29,7 +81,7 @@ val assert_spec_thm = store_thm(
         bsst_status := BST_AssertionViolated;
         bsst_pcond := BExp_BinExp BIExp_And pre
                  (BExp_UnaryExp BIExp_Not cond)|>})) ==>
-  (IS_BIR_CONTRADICTION (BExp_BinExp BIExp_And pre
+  (birs_pcondinf (BExp_BinExp BIExp_And pre
                  (BExp_UnaryExp BIExp_Not cond))) ==>
   (symb_hl_step_in_L_sound (bir_symb_rec_sbir bprog)
     (sys, L, IMAGE birs_symb_to_symbst {
@@ -38,7 +90,31 @@ val assert_spec_thm = store_thm(
         bsst_status := status;
         bsst_pcond := pre|>}))
 ``,
-  cheat
+  REPEAT STRIP_TAC >>
+  IMP_RES_TAC  symb_rulesTheory.symb_rule_INF_thm >>
+  PAT_X_ASSUM ``!x. A`` (ASSUME_TAC o SPEC ``birs_symb_to_symbst <|bsst_pc := lbl2; bsst_environ := env2;
+                  bsst_status := BST_AssertionViolated;
+                  bsst_pcond :=
+                    BExp_BinExp BIExp_And pre (BExp_UnaryExp BIExp_Not cond')|>``) >>
+
+  FULL_SIMP_TAC (std_ss++birs_state_ss) [IMAGE_INSERT, IMAGE_EMPTY, birs_symb_to_symbst_def] >>
+
+  `symb_pcondinf (bir_symb_rec_sbir bprog)
+          (SymbSymbSt lbl2 env2
+             (BExp_BinExp BIExp_And pre (BExp_UnaryExp BIExp_Not cond'))
+             BST_AssertionViolated)` by (
+    METIS_TAC [birs_pcondinf_thm, symb_symbst_pcond_def]
+  ) >>
+
+  `BExp_BinExp BIExp_And pre cond' <>
+   BExp_BinExp BIExp_And pre (BExp_UnaryExp BIExp_Not cond')` by (
+    FULL_SIMP_TAC (std_ss++holBACore_ss) [] >>
+    cheat
+  ) >>
+
+  FULL_SIMP_TAC (std_ss++symb_TYPES_ss) [DIFF_INSERT, DIFF_EMPTY, DELETE_INSERT, EMPTY_DELETE] >>
+
+  cheat (* TODO: use rule of consequence to drop BIR pcond conjunct *)
 );
 
 val symb_rule_SUBST_SING_thm = prove(``
